Remove generalization over Readers/Writers

runtime/test/tree_test.ml
@@ -14,8 +14,8 @@ let test_width max_height width =
   let rec loop i =
     if i < max_height
     then (test_serialize_deserialize (make false i width)
-                                     tree_serialize_iostream_top
-                                     (fun w -> match tree_deserialize_iostream_top w with
+                                     tree_serialize_top
+                                     (fun w -> match tree_deserialize_top w with
                                                | Some p -> p
                                                | None -> failwith "Deserialization failed")
                                      (fun _ -> Printf.printf "height %d, width %d"
@@ -34,7 +34,7 @@ let space_main () =
   let max_height = 10 in
   let rec loop i =
     if i < max_height
-    then (compare_cheerios_marshal_space (fun n -> make false n 2) (tree_serialize_iostream_top) i;
+    then (compare_cheerios_marshal_space (fun n -> make false n 2) (tree_serialize_top) i;
           loop (i + 1))
   in
   print_string "\nSpace usage tests...\n";
@@ -44,8 +44,8 @@ let bench_main () =
   print_string "\nBenchmarks...\n";
   compare_time_loop (fun n -> make false n 2)
                     20 1 10
-                    tree_serialize_iostream_top
-                    (fun w -> match tree_deserialize_iostream_top w with
+                    tree_serialize_top
+                    (fun w -> match tree_deserialize_top w with
                               | Some p -> p
                               | None -> failwith "Deserialization failed")
                     
