core/Combinators.v
@@ -3,10 +3,12 @@ Import ListNotations.
 Require Vector String.
 
 Require Import Cheerios.BasicSerializers.
+Require Import Cheerios.Core.
 Require Import Cheerios.DeserializerMonad.
-
 Require Import Cheerios.Tactics.
 Require Import Cheerios.Types.
+
+Import DeserializerNotations.
 
 (* These functions are either missing obvious implicits, or have
    implicit arguments that are not marked "maximally inserted", which
@@ -17,293 +19,282 @@ Arguments option_map {_ _} _ _.
 Arguments Vector.nil {_}.
 Arguments Vector.cons {_} _ {_} _.
 
-Module Combinators
-       (Writer : WRITER)
-       (Reader : READER)
-       (RWClass : SERIALIZERCLASS Writer Reader).
-  (* This section gives instances for various type constructors, including pairs
+(* This section gives instances for various type constructors, including pairs
     and lists. *)
-  Module RWBasic := BasicSerializers Writer Reader RWClass.
-  Export RWClass.
-  Export RWBasic.
 
-  Section BasicCombinators.
-    Variables A B : Type.
-    Variable sA : Serializer A.
-    Variable sB : Serializer B.
+Section BasicCombinators.
+  Variables A B : Type.
+  Variable sA : Serializer A.
+  Variable sB : Serializer B.
 
-    Definition bool_Serializer : Serializer bool :=
-      RWBasic.bool_Serializer.
-    
-    Definition option_serialize (x : option A) : Writer.t :=
-      match x with
-      | Some a => Writer.append (fun _ => serialize true)
-                                (fun _ => serialize a)
-      | None => serialize false
+  Definition option_serialize (x : option A) : IOStreamWriter.t :=
+    match x with
+    | Some a => IOStreamWriter.append (fun _ => serialize true)
+                              (fun _ => serialize a)
+    | None => serialize false
+    end.
+
+  Definition option_deserialize : ByteListReader.t (option A) :=
+    b <- deserialize ;;
+      match b with
+      | true => Some <$> deserialize
+      | false => ByteListReader.ret None
       end.
 
-    Definition option_deserialize : Reader.t (option A) :=
+  Lemma option_serialize_deserialize_id :
+    serialize_deserialize_id_spec option_serialize option_deserialize.
+  Proof.
+    intros.
+    unfold option_serialize, option_deserialize.
+    destruct a;
+      repeat (cheerios_crush; simpl).
+  Qed.
+
+  Global Instance option_Serializer : Serializer (option A).
+  Proof.
+    exact {| serialize := option_serialize;
+             deserialize := option_deserialize;
+             serialize_deserialize_id := option_serialize_deserialize_id |}.
+  Qed.
+
+
+  Definition pair_serialize (x : A * B) : IOStreamWriter.t :=
+    let (a, b) := x in IOStreamWriter.append (fun _ => serialize a)
+                                     (fun _ => serialize b).
+
+  Definition pair_deserialize : ByteListReader.t (A * B) :=
+    a <- deserialize ;;
       b <- deserialize ;;
-        match b with
-        | true => Some <$> deserialize
-        | false => Reader.ret None
-        end.
+      ByteListReader.ret (a, b).
 
-    Lemma option_serialize_deserialize_id :
-      serialize_deserialize_id_spec option_serialize option_deserialize.
-    Proof.
-      intros.
-      unfold option_serialize, option_deserialize.
-      destruct a;
-        repeat (cheerios_crush; simpl).
-    Qed.
+  Lemma pair_serialize_deserialize_id :
+    serialize_deserialize_id_spec pair_serialize pair_deserialize.
+  Proof.
+    intros.
+    unfold pair_serialize, pair_deserialize.
+    destruct a.
+    cheerios_crush.
+  Qed.
 
-    Global Instance option_Serializer : Serializer (option A).
-    Proof.
-      exact {| serialize := option_serialize;
-               deserialize := option_deserialize;
-               serialize_deserialize_id := option_serialize_deserialize_id |}.
-    Qed.
+  Global Instance pair_Serializer : Serializer (A * B).
+  Proof.
+    exact {| serialize := pair_serialize;
+             deserialize := pair_deserialize;
+             serialize_deserialize_id := pair_serialize_deserialize_id |}.
+  Qed.
 
-    
-    Definition pair_serialize (x : A * B) : Writer.t :=
-      let (a, b) := x in Writer.append (fun _ => serialize a)
-                                       (fun _ => serialize b).
-    
-    Definition pair_deserialize : Reader.t (A * B) :=
-      a <- deserialize ;;
-        b <- deserialize ;;
-        Reader.ret (a, b).
+  Definition sum_serialize (x : A + B) : IOStreamWriter.t :=
+    match x with
+    | inl a => IOStreamWriter.append (fun _ => serialize true)
+                             (fun _ => serialize a)
+    | inr b => IOStreamWriter.append (fun _ => serialize false)
+                             (fun _ => serialize b)
+    end.
 
-    Lemma pair_serialize_deserialize_id :
-      serialize_deserialize_id_spec pair_serialize pair_deserialize.
-    Proof.
-      intros.
-      unfold pair_serialize, pair_deserialize.
-      destruct a.
+  Definition sum_deserialize : ByteListReader.t (A + B) :=
+    b <- deserialize ;;
+      match b with
+      | true => inl <$> deserialize
+      | false => inr <$> deserialize
+      end.
+
+  Lemma sum_serialize_deserialize_id :
+    serialize_deserialize_id_spec sum_serialize sum_deserialize.
+  Proof.
+    unfold sum_serialize, sum_deserialize.
+    destruct a; cheerios_crush.
+  Qed.
+
+  Global Instance sum_Serializer : Serializer (A + B).
+  Proof.
+    exact {| serialize := sum_serialize;
+             deserialize := sum_deserialize;
+             serialize_deserialize_id := sum_serialize_deserialize_id
+          |}.
+  Qed.
+
+  Fixpoint list_serialize_rec (l : list A) : IOStreamWriter.t :=
+    match l with
+    | [] => IOStreamWriter.empty
+    | a :: l' => IOStreamWriter.append (fun _ => serialize a)
+                               (fun _ => list_serialize_rec l')
+    end.
+
+  Fixpoint list_serialize_aux (l : list A) (acc : IOStreamWriter.t) : IOStreamWriter.t :=
+    match l with
+    | [] => acc
+    | a :: l' =>  list_serialize_aux l' (IOStreamWriter.append (fun _ => acc)
+                                                       (fun _ => serialize a))
+    end.
+
+  Lemma list_serialize_rec'_aux : forall l acc,
+      IOStreamWriter.unwrap (list_serialize_aux l acc) =
+      IOStreamWriter.unwrap (IOStreamWriter.append (fun _ => acc)
+                                   (fun _ => list_serialize_rec l)).
+  Proof.
+    intros l.
+    induction l; intros.
+    - simpl.
       cheerios_crush.
-    Qed.
-
-    Global Instance pair_Serializer : Serializer (A * B).
-    Proof.
-      exact {| serialize := pair_serialize;
-               deserialize := pair_deserialize;
-               serialize_deserialize_id := pair_serialize_deserialize_id |}.
-    Qed.
-
-    Definition sum_serialize (x : A + B) : Writer.t :=
-      match x with
-      | inl a => Writer.append (fun _ => serialize true)
-                               (fun _ => serialize a)
-      | inr b => Writer.append (fun _ => serialize false)
-                               (fun _ => serialize b)
-      end.
-
-    Definition sum_deserialize : Reader.t (A + B) :=
-      b <- deserialize ;;
-        match b with
-        | true => inl <$> deserialize
-        | false => inr <$> deserialize
-        end.
-
-    Lemma sum_serialize_deserialize_id :
-      serialize_deserialize_id_spec sum_serialize sum_deserialize.
-    Proof.
-      unfold sum_serialize, sum_deserialize.
-      destruct a; cheerios_crush.
-    Qed.
-
-    Global Instance sum_Serializer : Serializer (A + B).
-    Proof.
-      exact {| serialize := sum_serialize;
-               deserialize := sum_deserialize;
-               serialize_deserialize_id := sum_serialize_deserialize_id
-            |}.
-    Qed.
-    
-    Fixpoint list_serialize_rec (l : list A) : Writer.t :=
-      match l with
-      | [] => Writer.empty
-      | a :: l' => Writer.append (fun _ => serialize a)
-                                 (fun _ => list_serialize_rec l')
-      end.
-
-    Fixpoint list_serialize_aux (l : list A) (acc : Writer.t) : Writer.t :=
-      match l with
-      | [] => acc
-      | a :: l' =>  list_serialize_aux l' (Writer.append (fun _ => acc)
-                                                         (fun _ => serialize a))
-      end.
-
-    Lemma list_serialize_rec'_aux : forall l acc,
-        Writer.unwrap (list_serialize_aux l acc) =
-        Writer.unwrap (Writer.append (fun _ => acc)
-                                     (fun _ => list_serialize_rec l)).
-    Proof.
-      intros l.
-      induction l; intros.
-      - simpl.
-        cheerios_crush.
-        now rewrite app_nil_r.
-      - unfold list_serialize_aux. fold list_serialize_aux.
-        rewrite IHl.
-        unfold list_serialize_rec at 2.
-        fold list_serialize_rec.
-        cheerios_crush.
-    Qed.
-
-    Definition list_serialize_rec' (l : list A) : Writer.t :=
-      list_serialize_aux l Writer.empty.
-
-    Definition list_serialize (l : list A) : Writer.t :=
-      Writer.append (fun _ => serialize (length l))
-                    (fun _ => list_serialize_rec l).
-
-    Definition list_serialize' (l : list A) : Writer.t :=
-        Writer.append (fun _ => serialize (length l))
-                      (fun _ => list_serialize_rec' l).
-
-    Fixpoint list_deserialize_rec (n : nat) : Reader.t (list A) :=
-      match n with
-      | 0 => Reader.ret []
-      | S n' => cons <$> deserialize <*> list_deserialize_rec n'
-      end.
-
-    Definition list_deserialize : Reader.t (list A) :=
-      deserialize >>= list_deserialize_rec.
-
-    Lemma list_serialize_deserialize_id_rec :
-      forall l bin, Reader.unwrap (list_deserialize_rec (length l))
-                                  (Writer.unwrap (list_serialize_rec l) ++ bin)
-                    = Some(l, bin).
-    Proof.
-      intros.
-      unfold list_serialize_rec.
-      cheerios_crush. simpl.
-      induction l;
-        simpl;
-        cheerios_crush.
-      unfold DeserializerMonad.sequence.
+      now rewrite app_nil_r.
+    - unfold list_serialize_aux. fold list_serialize_aux.
       rewrite IHl.
+      unfold list_serialize_rec at 2.
+      fold list_serialize_rec.
       cheerios_crush.
-    Qed.
+  Qed.
 
-    Lemma list_serialize_deserialize_id :
-      serialize_deserialize_id_spec list_serialize list_deserialize.
-    Proof.
-      unfold list_serialize, list_deserialize.
+  Definition list_serialize_rec' (l : list A) : IOStreamWriter.t :=
+    list_serialize_aux l IOStreamWriter.empty.
+
+  Definition list_serialize (l : list A) : IOStreamWriter.t :=
+    IOStreamWriter.append (fun _ => serialize (length l))
+                  (fun _ => list_serialize_rec l).
+
+  Definition list_serialize' (l : list A) : IOStreamWriter.t :=
+    IOStreamWriter.append (fun _ => serialize (length l))
+                  (fun _ => list_serialize_rec' l).
+
+  Fixpoint list_deserialize_rec (n : nat) : ByteListReader.t (list A) :=
+    match n with
+    | 0 => ByteListReader.ret []
+    | S n' => cons <$> deserialize <*> list_deserialize_rec n'
+    end.
+
+  Definition list_deserialize : ByteListReader.t (list A) :=
+    deserialize >>= list_deserialize_rec.
+
+  Lemma list_serialize_deserialize_id_rec :
+    forall l bin, ByteListReader.unwrap (list_deserialize_rec (length l))
+                                (IOStreamWriter.unwrap (list_serialize_rec l) ++ bin)
+                  = Some(l, bin).
+  Proof.
+    intros.
+    unfold list_serialize_rec.
+    cheerios_crush. simpl.
+    induction l;
+      simpl;
       cheerios_crush.
-      now rewrite list_serialize_deserialize_id_rec.
-    Qed.
+    unfold DeserializerMonad.sequence.
+    rewrite IHl.
+    cheerios_crush.
+  Qed.
 
-    Lemma list_serialize'_deserialize_id_rec :
-      forall l bin, Reader.unwrap (list_deserialize_rec (length l))
-                                  (Writer.unwrap (list_serialize_rec' l) ++ bin)
-                    = Some(l, bin).
-    Proof.
-      intros.
-      unfold list_serialize_rec'.
-      rewrite list_serialize_rec'_aux.
-      cheerios_crush. simpl.
-      now rewrite list_serialize_deserialize_id_rec.
-    Qed.
+  Lemma list_serialize_deserialize_id :
+    serialize_deserialize_id_spec list_serialize list_deserialize.
+  Proof.
+    unfold list_serialize, list_deserialize.
+    cheerios_crush.
+    now rewrite list_serialize_deserialize_id_rec.
+  Qed.
 
-    Lemma list_serialize'_deserialize_id :
-      serialize_deserialize_id_spec list_serialize' list_deserialize.
-    Proof.
-      unfold list_serialize', list_deserialize.
+  Lemma list_serialize'_deserialize_id_rec :
+    forall l bin, ByteListReader.unwrap (list_deserialize_rec (length l))
+                                (IOStreamWriter.unwrap (list_serialize_rec' l) ++ bin)
+                  = Some(l, bin).
+  Proof.
+    intros.
+    unfold list_serialize_rec'.
+    rewrite list_serialize_rec'_aux.
+    cheerios_crush. simpl.
+    now rewrite list_serialize_deserialize_id_rec.
+  Qed.
+
+  Lemma list_serialize'_deserialize_id :
+    serialize_deserialize_id_spec list_serialize' list_deserialize.
+  Proof.
+    unfold list_serialize', list_deserialize.
+    cheerios_crush.
+    now rewrite list_serialize'_deserialize_id_rec.
+  Qed.
+
+
+  Global Instance list_Serializer : Serializer (list A).
+  Proof.
+    exact {| serialize := list_serialize;
+             deserialize := list_deserialize;
+             serialize_deserialize_id := list_serialize_deserialize_id
+          |}.
+  Qed.
+
+  Fixpoint vector_serialize {n} (v : Vector.t A n) : IOStreamWriter.t :=
+    match v with
+    | Vector.nil => IOStreamWriter.empty
+    | Vector.cons a v' => IOStreamWriter.append (fun _ => serialize a)
+                                        (fun _ => vector_serialize v')
+    end.
+
+  Fixpoint vector_deserialize {n} : ByteListReader.t (Vector.t A n) :=
+    match n as n0 return ByteListReader.t (Vector.t A n0) with
+    | 0 => ByteListReader.ret Vector.nil
+    | S n' => a <- deserialize ;;
+                v <- vector_deserialize ;;
+                ByteListReader.ret (Vector.cons a v)
+    end.
+
+  Lemma vector_serialize_deserialize_id :
+    forall n, serialize_deserialize_id_spec vector_serialize (@vector_deserialize n).
+  Proof.
+    induction n; intros.
+    - destruct a using Vector.case0. auto. unfold vector_serialize,  vector_deserialize.
       cheerios_crush.
-      now rewrite list_serialize'_deserialize_id_rec.
-    Qed.
+    - destruct a using Vector.caseS'.
+      simpl.
+      cheerios_crush.
+      rewrite IHn.
+      cheerios_crush.
+  Qed.
+
+  Global Instance vector_Serializer n : Serializer (Vector.t A n).
+  Proof.
+    exact {| serialize := vector_serialize;
+             deserialize := vector_deserialize;
+             serialize_deserialize_id := vector_serialize_deserialize_id n
+          |}.
+  Qed.
+End BasicCombinators.
 
 
-    Global Instance list_Serializer : Serializer (list A).
-    Proof.
-      exact {| serialize := list_serialize;
-               deserialize := list_deserialize;
-               serialize_deserialize_id := list_serialize_deserialize_id
-            |}.
-    Qed.
-
-    Fixpoint vector_serialize {n} (v : Vector.t A n) : Writer.t :=
-      match v with
-      | Vector.nil => Writer.empty
-      | Vector.cons a v' => Writer.append (fun _ => serialize a)
-                                          (fun _ => vector_serialize v')
-      end.
-
-    Fixpoint vector_deserialize {n} : Reader.t (Vector.t A n) :=
-      match n as n0 return Reader.t (Vector.t A n0) with
-      | 0 => Reader.ret Vector.nil
-      | S n' => a <- deserialize ;;
-                  v <- vector_deserialize ;;
-                  Reader.ret (Vector.cons a v)
-      end.
-
-    Lemma vector_serialize_deserialize_id :
-      forall n, serialize_deserialize_id_spec vector_serialize (@vector_deserialize n).
-    Proof.
-      induction n; intros.
-      - destruct a using Vector.case0. auto. unfold vector_serialize,  vector_deserialize.
-        cheerios_crush.
-      - destruct a using Vector.caseS'.
-        simpl.
-        cheerios_crush.
-        rewrite IHn.
-        cheerios_crush.
-    Qed.
-
-    Global Instance vector_Serializer n : Serializer (Vector.t A n).
-    Proof.
-      exact {| serialize := vector_serialize;
-               deserialize := vector_deserialize;
-               serialize_deserialize_id := vector_serialize_deserialize_id n
-            |}.
-    Qed.
-  End BasicCombinators.
-
-
-    (* This has to go here because it depends on having a serializer for
+(* This has to go here because it depends on having a serializer for
    lists available. *)
 
-    Fixpoint string_to_list s :=
-      match s with
-      | String.EmptyString => nil
-      | String.String c s' => c :: (string_to_list s')
-      end.
+Fixpoint string_to_list s :=
+  match s with
+  | String.EmptyString => nil
+  | String.String c s' => c :: (string_to_list s')
+  end.
 
-    Fixpoint list_to_string l :=
-      match l with
-      | nil => String.EmptyString
-      | h::l' => String.String h (list_to_string l')
-      end.
+Fixpoint list_to_string l :=
+  match l with
+  | nil => String.EmptyString
+  | h::l' => String.String h (list_to_string l')
+  end.
 
-    Lemma string_to_list_to_string :
-      forall s, list_to_string (string_to_list s) = s.
-    Proof.
-      induction s; auto; simpl.
-      now rewrite IHs.
-    Qed.
+Lemma string_to_list_to_string :
+  forall s, list_to_string (string_to_list s) = s.
+Proof.
+  induction s; auto; simpl.
+  now rewrite IHs.
+Qed.
 
-    Definition string_serialize (s : String.string) :=
-      serialize (string_to_list s).
+Definition string_serialize (s : String.string) :=
+  serialize (string_to_list s).
 
-    Definition string_deserialize : Reader.t String.string :=
-      list_to_string <$> deserialize.
+Definition string_deserialize : ByteListReader.t String.string :=
+  list_to_string <$> deserialize.
 
-    Lemma string_serialize_deserialize_id :
-      serialize_deserialize_id_spec string_serialize string_deserialize.
-    Proof.
-      unfold string_deserialize, string_serialize.
-      cheerios_crush.
-      now rewrite string_to_list_to_string.
-    Qed.
+Lemma string_serialize_deserialize_id :
+  serialize_deserialize_id_spec string_serialize string_deserialize.
+Proof.
+  unfold string_deserialize, string_serialize.
+  cheerios_crush.
+  now rewrite string_to_list_to_string.
+Qed.
 
-    Instance string_Serializer : Serializer String.string.
-    Proof.
-      exact {| serialize := string_serialize;
-               deserialize := string_deserialize;
-               serialize_deserialize_id := string_serialize_deserialize_id
-            |}.
-    Qed.
-End Combinators.
+Instance string_Serializer : Serializer String.string.
+Proof.
+  exact {| serialize := string_serialize;
+           deserialize := string_deserialize;
+           serialize_deserialize_id := string_serialize_deserialize_id
+        |}.
+Qed.
