core/BasicSerializers.v
@@ -4,423 +4,410 @@ Import ListNotations.
 From StructTact Require Import StructTactics Fin.
 Require Fin Ascii.
 
+Require Import Cheerios.Core.
 Require Import Cheerios.DeserializerMonad.
 Require Import Cheerios.Tactics.
 Require Import Cheerios.Types.
-Require Import Cheerios.IOStream.
 
-Module BasicSerializers
-       (Writer : WRITER)
-       (Reader : READER)
-       (RWClass : SERIALIZERCLASS Writer Reader).
-  Module WRewrite := WriterRewrite Writer.
-  Module RRewrite := ReaderRewrite Reader.
-  Export WRewrite.
-  Export RRewrite.
+Import DeserializerNotations.
 
-  Module DeserializerMonad := DeserializerMonad Reader.
-  Export DeserializerMonad.
-  Export DeserializerNotations.
+Lemma byte_serialize_deserialize_id :
+  serialize_deserialize_id_spec IOStreamWriter.putByte ByteListReader.getByte.
+Proof. cheerios_crush. Qed.
 
-  Import RWClass.
+Instance byte_Serializer : Serializer byte :=
+  {| serialize := IOStreamWriter.putByte;
+     deserialize := ByteListReader.getByte;
+     serialize_deserialize_id := byte_serialize_deserialize_id |}.
 
-  Lemma byte_serialize_deserialize_id :
-    serialize_deserialize_id_spec Writer.putByte Reader.getByte.
-  Proof. cheerios_crush. Qed.
+Lemma byte_unwrap : forall b, IOStreamWriter.unwrap (serialize b) = [b].
+Proof.
+  unfold serialize. simpl.
+  cheerios_crush.
+Qed.
 
-  Instance byte_Serializer : Serializer byte :=
-    {| serialize := Writer.putByte;
-       deserialize := Reader.getByte;
-       serialize_deserialize_id := byte_serialize_deserialize_id |}.
+Hint Rewrite byte_unwrap : cheerios.
 
-  Lemma byte_unwrap : forall b, Writer.unwrap (serialize b) = [b].
-  Proof.
-    unfold serialize. simpl.
-    cheerios_crush.
-  Qed.
+Definition bool_serialize (b : bool) : IOStreamWriter.t :=
+  if b then serialize x01 else serialize x00.
 
-  Hint Rewrite byte_unwrap : cheerios.
-
-  Definition bool_serialize (b : bool) : Writer.t :=
-    if b then serialize x01 else serialize x00.
-
-  Definition bool_deserialize :=
-    b <- deserialize ;;
-      match b with
-      | x00 => Reader.ret false
-      | x01 => Reader.ret true
-      | _ => Reader.error
-      end.
-
-  Lemma bool_serialize_deserialize_id :
-    serialize_deserialize_id_spec bool_serialize bool_deserialize.
-  Proof.
-    intros.
-    unfold bool_serialize, bool_deserialize.
-    destruct a;
-      cheerios_crush; simpl; cheerios_crush.
-  Qed.
-
-  Global Instance bool_Serializer : Serializer bool.
-  Proof.
-    exact {| serialize := bool_serialize;
-             deserialize := bool_deserialize;
-             serialize_deserialize_id := bool_serialize_deserialize_id |}.
-  Qed.
-
-  (* this needs to go here because we need the bool_Serializer instance *)
-  Lemma fold_append_unwrap :
-    forall {S A : Type}
-           (f : byte -> S -> fold_state S A) (s : S)
-           (b : byte) (tail : Writer.t) (bin : list byte),
-      Reader.unwrap (Reader.fold f s)
-                    (Writer.unwrap (Writer.append
-                                      (fun _ => (serialize b))
-                                      (fun _ => tail)) ++ bin) =
-      match f b s with
-      | Done a => Some(a, Writer.unwrap tail ++ bin)
-      | More s => Reader.unwrap (Reader.fold f s)
-                                (Writer.unwrap tail ++ bin)
-      | Error => None
-      end.
-  Proof.
-    cheerios_crush.
-  Qed.
-
-  Lemma fold_append_unwrap' :
-    forall {S A : Type}
-           (f : byte -> S -> fold_state S A) (s : S)
-           (b : byte) (tail : Writer.t) (bin : list byte),
-      Reader.unwrap (Reader.fold f s)
-                    (Writer.unwrap (Writer.append
-                                      (fun _ => Writer.putByte b)
-                                      (fun _ => tail)) ++ bin) =
-      match f b s with
-      | Done a => Some(a, Writer.unwrap tail ++ bin)
-      | More s => Reader.unwrap (Reader.fold f s)
-                                (Writer.unwrap tail ++ bin)
-      | Error => None
-      end.
-  Proof.
-    cheerios_crush.
-  Qed.
-  Hint Rewrite @fold_append_unwrap @fold_append_unwrap' : cheerios.
-
-
-  Inductive le_pos (p : positive) : positive -> Prop :=
-  | le_p : le_pos p p
-  | le_xI : forall p2, le_pos p p2 -> le_pos p (xI p2)
-  | le_xO : forall p2, le_pos p p2 -> le_pos p (xO p2).
-
-  Section PositiveInductionPrinciple.
-    Variable P : positive -> Prop.
-
-    Lemma strongind_pos_aux :
-      P xH ->
-      (forall q, ((forall p, le_pos p q -> P p) -> P (xI q)) /\
-                 ((forall p, le_pos p q -> P p) -> P (xO q))) ->
-      (forall q, (forall p, le_pos p q -> P p)).
-    Proof.
-      induction q;
-        intros;
-        inversion H1;
-        auto;
-        apply H0;
-        apply IHq.
-    Qed.
-
-    Lemma weaken_pos :
-      (forall q, (forall p, le_pos p q -> P p)) -> forall p, P p.
-    Proof.
-      intros.
-      apply (H p p).
-      constructor.
-    Qed.
-
-    Theorem strongind_pos :
-      P xH ->
-      (forall q, ((forall p, le_pos p q -> P p) -> P (xI q)) /\
-                 ((forall p, le_pos p q -> P p) -> P (xO q))) ->
-      forall p, P p.
-    Proof.
-      intros.
-      apply weaken_pos.
-      now apply strongind_pos_aux.
-    Qed.
-  End PositiveInductionPrinciple.
-
-  Local Open Scope char_scope.
-
-  Fixpoint positive_serialize p :=
-    match p with
-    | xI (xI (xI p)) => Writer.append (fun _ => serialize x0e)
-                                      (fun _ => positive_serialize p)
-    | xI (xI (xO p)) => Writer.append (fun _ => serialize x0d)
-                                      (fun _ => positive_serialize p)
-    | xI (xO (xI p)) => Writer.append (fun _ => serialize x0c)
-                                      (fun _ => positive_serialize p)
-    | xI (xO (xO p)) => Writer.append (fun _ => serialize x0b)
-                                      (fun _ => positive_serialize p)
-    | xO (xI (xI p)) => Writer.append (fun _ => serialize x0a)
-                                      (fun _ => positive_serialize p)
-    | xO (xI (xO p)) => Writer.append (fun _ => serialize x09)
-                                      (fun _ => positive_serialize p)
-    | xO (xO (xI p)) => Writer.append (fun _ => serialize x08)
-                                      (fun _ => positive_serialize p)
-    | xO (xO (xO p)) => Writer.append (fun _ => serialize x07)
-                                      (fun _ => positive_serialize p)
-    | xI (xI p) => Writer.append (fun _ => serialize x06)
-                                 (fun _ => positive_serialize p)
-    | xI (xO p) => Writer.append (fun _ => serialize x05)
-                                 (fun _ => positive_serialize p)
-    | xO (xI p) => Writer.append (fun _ => serialize x04)
-                                 (fun _ => positive_serialize p)
-    | xO (xO p) => Writer.append (fun _ => serialize x03)
-                                 (fun _ => positive_serialize p)
-    | xI p => Writer.append (fun _ => serialize x02)
-                            (fun _ => positive_serialize p)
-    | xO p => Writer.append (fun _ => serialize x01)
-                            (fun _ => positive_serialize p)
-    | XH => serialize x00
-    end.
-
-  Definition positive_deserialize_step
-             (b : byte)
-             (s : positive -> positive) := 
+Definition bool_deserialize :=
+  b <- deserialize ;;
     match b with
-    | x0e => More (fun p => s (xI (xI (xI p))))
-    | x0d => More (fun p => s (xI (xI (xO p))))
-    | x0c => More (fun p => s (xI (xO (xI p))))
-    | x0b => More (fun p => s (xI (xO (xO p))))
-    | x0a => More (fun p => s (xO (xI (xI p))))
-    | x09 => More (fun p => s (xO (xI (xO p))))
-    | x08 => More (fun p =>  s (xO (xO (xI p))))
-    | x07 => More (fun p => s (xO (xO (xO p))))
-    | x06 => More (fun p => s (xI (xI p)))
-    | x05 => More (fun p => s (xI (xO p)))
-    | x04 => More (fun p => s (xO (xI p)))
-    | x03 => More (fun p => s (xO (xO p)))
-    | x02 => More (fun p => s (xI p))
-    | x01 => More (fun p => s (xO p))
-    | x00 => Done (s xH)
-    | _ => Error
+    | x00 => ByteListReader.ret false
+    | x01 => ByteListReader.ret true
+    | _ => ByteListReader.error
     end.
 
-  Definition positive_step_aux p :=
-    forall (k : positive -> positive) (bytes : list byte),
-      Reader.unwrap (Reader.fold positive_deserialize_step k)
-                    (Writer.unwrap (positive_serialize p) ++ bytes)
-      = Some(k p, bytes).
+Lemma bool_serialize_deserialize_id :
+  serialize_deserialize_id_spec bool_serialize bool_deserialize.
+Proof.
+  intros.
+  unfold bool_serialize, bool_deserialize.
+  destruct a;
+    cheerios_crush; simpl; cheerios_crush.
+Qed.
 
-  Lemma positive_step :
-    forall (p : positive), positive_step_aux p.
+Instance bool_Serializer : Serializer bool.
+Proof.
+  exact {| serialize := bool_serialize;
+           deserialize := bool_deserialize;
+           serialize_deserialize_id := bool_serialize_deserialize_id |}.
+Qed.
+
+(* this needs to go here because we need the bool_Serializer instance *)
+Lemma fold_append_unwrap :
+  forall {S A : Type}
+         (f : byte -> S -> fold_state S A) (s : S)
+         (b : byte) (tail : IOStreamWriter.t) (bin : list byte),
+    ByteListReader.unwrap (ByteListReader.fold f s)
+                          (IOStreamWriter.unwrap (IOStreamWriter.append
+                                                    (fun _ => (serialize b))
+                                                    (fun _ => tail)) ++ bin) =
+    match f b s with
+    | Done a => Some(a, IOStreamWriter.unwrap tail ++ bin)
+    | More s => ByteListReader.unwrap (ByteListReader.fold f s)
+                                      (IOStreamWriter.unwrap tail ++ bin)
+    | Error => None
+    end.
+Proof.
+  cheerios_crush.
+Qed.
+
+Lemma fold_append_unwrap' :
+  forall {S A : Type}
+         (f : byte -> S -> fold_state S A) (s : S)
+         (b : byte) (tail : IOStreamWriter.t) (bin : list byte),
+    ByteListReader.unwrap (ByteListReader.fold f s)
+                          (IOStreamWriter.unwrap (IOStreamWriter.append
+                                                    (fun _ => IOStreamWriter.putByte b)
+                                                    (fun _ => tail)) ++ bin) =
+    match f b s with
+    | Done a => Some(a, IOStreamWriter.unwrap tail ++ bin)
+    | More s => ByteListReader.unwrap (ByteListReader.fold f s)
+                                      (IOStreamWriter.unwrap tail ++ bin)
+    | Error => None
+    end.
+Proof.
+  cheerios_crush.
+Qed.
+Hint Rewrite @fold_append_unwrap @fold_append_unwrap' : cheerios.
+
+
+Inductive le_pos (p : positive) : positive -> Prop :=
+| le_p : le_pos p p
+| le_xI : forall p2, le_pos p p2 -> le_pos p (xI p2)
+| le_xO : forall p2, le_pos p p2 -> le_pos p (xO p2).
+
+Section PositiveInductionPrinciple.
+  Variable P : positive -> Prop.
+
+  Lemma strongind_pos_aux :
+    P xH ->
+    (forall q, ((forall p, le_pos p q -> P p) -> P (xI q)) /\
+               ((forall p, le_pos p q -> P p) -> P (xO q))) ->
+    (forall q, (forall p, le_pos p q -> P p)).
   Proof.
-    apply strongind_pos; unfold positive_step_aux.
-    - unfold positive_serialize.
-      cheerios_crush.
-    - split;
-        intros;
-        try destruct q;
-        try destruct q;
-        simpl; cheerios_crush; simpl; rewrite H || cheerios_crush;
-          try reflexivity;
-          repeat constructor.
+    induction q;
+      intros;
+      inversion H1;
+      auto;
+      apply H0;
+      apply IHq.
   Qed.
 
-  Definition positive_deserialize :=
-    Reader.fold positive_deserialize_step (fun p => p).
-
-  Theorem positive_serialize_deserialize_id :
-    serialize_deserialize_id_spec positive_serialize
-                                  positive_deserialize.
+  Lemma weaken_pos :
+    (forall q, (forall p, le_pos p q -> P p)) -> forall p, P p.
   Proof.
     intros.
-    unfold positive_deserialize.
-    apply positive_step.
+    apply (H p p).
+    constructor.
   Qed.
 
-  Instance positive_Serializer : Serializer positive.
+  Theorem strongind_pos :
+    P xH ->
+    (forall q, ((forall p, le_pos p q -> P p) -> P (xI q)) /\
+               ((forall p, le_pos p q -> P p) -> P (xO q))) ->
+    forall p, P p.
   Proof.
-    exact ({| serialize := positive_serialize;
-              deserialize := positive_deserialize;
-              serialize_deserialize_id := positive_serialize_deserialize_id
-           |}).
+    intros.
+    apply weaken_pos.
+    now apply strongind_pos_aux.
   Qed.
+End PositiveInductionPrinciple.
+
+Local Open Scope char_scope.
+
+Fixpoint positive_serialize p :=
+  match p with
+  | xI (xI (xI p)) => IOStreamWriter.append (fun _ => serialize x0e)
+                                            (fun _ => positive_serialize p)
+  | xI (xI (xO p)) => IOStreamWriter.append (fun _ => serialize x0d)
+                                            (fun _ => positive_serialize p)
+  | xI (xO (xI p)) => IOStreamWriter.append (fun _ => serialize x0c)
+                                            (fun _ => positive_serialize p)
+  | xI (xO (xO p)) => IOStreamWriter.append (fun _ => serialize x0b)
+                                            (fun _ => positive_serialize p)
+  | xO (xI (xI p)) => IOStreamWriter.append (fun _ => serialize x0a)
+                                            (fun _ => positive_serialize p)
+  | xO (xI (xO p)) => IOStreamWriter.append (fun _ => serialize x09)
+                                            (fun _ => positive_serialize p)
+  | xO (xO (xI p)) => IOStreamWriter.append (fun _ => serialize x08)
+                                            (fun _ => positive_serialize p)
+  | xO (xO (xO p)) => IOStreamWriter.append (fun _ => serialize x07)
+                                            (fun _ => positive_serialize p)
+  | xI (xI p) => IOStreamWriter.append (fun _ => serialize x06)
+                                       (fun _ => positive_serialize p)
+  | xI (xO p) => IOStreamWriter.append (fun _ => serialize x05)
+                                       (fun _ => positive_serialize p)
+  | xO (xI p) => IOStreamWriter.append (fun _ => serialize x04)
+                                       (fun _ => positive_serialize p)
+  | xO (xO p) => IOStreamWriter.append (fun _ => serialize x03)
+                                       (fun _ => positive_serialize p)
+  | xI p => IOStreamWriter.append (fun _ => serialize x02)
+                                  (fun _ => positive_serialize p)
+  | xO p => IOStreamWriter.append (fun _ => serialize x01)
+                                  (fun _ => positive_serialize p)
+  | XH => serialize x00
+  end.
+
+Definition positive_deserialize_step
+           (b : byte)
+           (s : positive -> positive) :=
+  match b with
+  | x0e => More (fun p => s (xI (xI (xI p))))
+  | x0d => More (fun p => s (xI (xI (xO p))))
+  | x0c => More (fun p => s (xI (xO (xI p))))
+  | x0b => More (fun p => s (xI (xO (xO p))))
+  | x0a => More (fun p => s (xO (xI (xI p))))
+  | x09 => More (fun p => s (xO (xI (xO p))))
+  | x08 => More (fun p =>  s (xO (xO (xI p))))
+  | x07 => More (fun p => s (xO (xO (xO p))))
+  | x06 => More (fun p => s (xI (xI p)))
+  | x05 => More (fun p => s (xI (xO p)))
+  | x04 => More (fun p => s (xO (xI p)))
+  | x03 => More (fun p => s (xO (xO p)))
+  | x02 => More (fun p => s (xI p))
+  | x01 => More (fun p => s (xO p))
+  | x00 => Done (s xH)
+  | _ => Error
+  end.
+
+Definition positive_step_aux p :=
+  forall (k : positive -> positive) (bytes : list byte),
+    ByteListReader.unwrap (ByteListReader.fold positive_deserialize_step k)
+                          (IOStreamWriter.unwrap (positive_serialize p) ++ bytes)
+    = Some(k p, bytes).
+
+Lemma positive_step :
+  forall (p : positive), positive_step_aux p.
+Proof.
+  apply strongind_pos; unfold positive_step_aux.
+  - unfold positive_serialize.
+    cheerios_crush.
+  - split;
+      intros;
+      try destruct q;
+      try destruct q;
+      simpl; cheerios_crush; simpl; rewrite H || cheerios_crush;
+        try reflexivity;
+        repeat constructor.
+Qed.
+
+Definition positive_deserialize :=
+  ByteListReader.fold positive_deserialize_step (fun p => p).
+
+Theorem positive_serialize_deserialize_id :
+  serialize_deserialize_id_spec positive_serialize
+                                positive_deserialize.
+Proof.
+  intros.
+  unfold positive_deserialize.
+  apply positive_step.
+Qed.
+
+Instance positive_Serializer : Serializer positive.
+Proof.
+  exact ({| serialize := positive_serialize;
+            deserialize := positive_deserialize;
+            serialize_deserialize_id := positive_serialize_deserialize_id
+         |}).
+Qed.
 
 
-  (* This is the first example of a "typical" serializer: it combines more
+(* This is the first example of a "typical" serializer: it combines more
    primitive serializers (in this case, just for byte and positive) together in
    order to serialize a Z. *)
-  Definition Z_serialize (z : Z) : Writer.t :=
-    match z with
-    | Z0 => serialize x00
-    | Zpos p => Writer.append (fun _ => serialize x01)
-                              (fun _ => serialize p)
-    | Zneg p => Writer.append (fun _ => serialize x02)
-                              (fun _ => serialize p)
-    end.
+Definition Z_serialize (z : Z) : IOStreamWriter.t :=
+  match z with
+  | Z0 => serialize x00
+  | Zpos p => IOStreamWriter.append (fun _ => serialize x01)
+                                    (fun _ => serialize p)
+  | Zneg p => IOStreamWriter.append (fun _ => serialize x02)
+                                    (fun _ => serialize p)
+  end.
 
-  Definition Z_deserialize : Reader.t Z :=
-    tag <- deserialize ;;
-        match tag with
-        | x02 => Zneg <$> deserialize
-        | x01 => Zpos <$> deserialize
-        | x00 => Reader.ret Z0
-        | _ => Reader.error
-        end.
+Definition Z_deserialize : ByteListReader.t Z :=
+  tag <- deserialize ;;
+      match tag with
+      | x02 => Zneg <$> deserialize
+      | x01 => Zpos <$> deserialize
+      | x00 => ByteListReader.ret Z0
+      | _ => ByteListReader.error
+      end.
 
-  (* This proof is typical for serializing an algebraic datatype. Unfold the
+(* This proof is typical for serializing an algebraic datatype. Unfold the
    serializer and deserializer, then do a case analysis and call
    serialize_deserialize_id_crush. *)
-  Lemma Z_serialize_deserialize_id :
-    serialize_deserialize_id_spec Z_serialize Z_deserialize.
-  Proof.
-    intros.
-    unfold Z_serialize, Z_deserialize.
-    destruct a;
-      repeat (cheerios_crush; simpl).
-  Qed.
+Lemma Z_serialize_deserialize_id :
+  serialize_deserialize_id_spec Z_serialize Z_deserialize.
+Proof.
+  intros.
+  unfold Z_serialize, Z_deserialize.
+  destruct a;
+    repeat (cheerios_crush; simpl).
+Qed.
 
-  Instance Z_Serializer : Serializer Z :=
-    {| serialize := Z_serialize;
-       deserialize := Z_deserialize;
-       serialize_deserialize_id := Z_serialize_deserialize_id
-    |}.
+Instance Z_Serializer : Serializer Z :=
+  {| serialize := Z_serialize;
+     deserialize := Z_deserialize;
+     serialize_deserialize_id := Z_serialize_deserialize_id
+  |}.
 
-  Definition N_serialize n :=
-    match n with
-    | N0 => serialize false
-    | Npos p => Writer.append (fun _ => serialize true)
-                              (fun _ => serialize p)
-    end.
+Definition N_serialize n :=
+  match n with
+  | N0 => serialize false
+  | Npos p => IOStreamWriter.append (fun _ => serialize true)
+                                    (fun _ => serialize p)
+  end.
 
-  Definition N_deserialize : Reader.t N :=
-    tag <- deserialize ;;
-        match tag with
-        | false => Reader.ret N0
-        | true => Npos <$> deserialize
-        end.
+Definition N_deserialize : ByteListReader.t N :=
+  tag <- deserialize ;;
+      match tag with
+      | false => ByteListReader.ret N0
+      | true => Npos <$> deserialize
+      end.
 
-  Lemma N_serialize_deserialize_id :
-    serialize_deserialize_id_spec N_serialize N_deserialize.
-  Proof.
-    intros.
-    unfold N_serialize, N_deserialize.
-    destruct a;
-      repeat (cheerios_crush; simpl).
-  Qed.
+Lemma N_serialize_deserialize_id :
+  serialize_deserialize_id_spec N_serialize N_deserialize.
+Proof.
+  intros.
+  unfold N_serialize, N_deserialize.
+  destruct a;
+    repeat (cheerios_crush; simpl).
+Qed.
 
-  Instance N_Serializer : Serializer N :=
-    {| serialize := N_serialize;
-       deserialize := N_deserialize;
-       serialize_deserialize_id := N_serialize_deserialize_id
-    |}.
+Instance N_Serializer : Serializer N :=
+  {| serialize := N_serialize;
+     deserialize := N_deserialize;
+     serialize_deserialize_id := N_serialize_deserialize_id
+  |}.
 
-  (* The other main way to define a serializer is to use an isomorphism to another
+(* The other main way to define a serializer is to use an isomorphism to another
    type that is already serializable. *)
-  Definition nat_serialize n : Writer.t := serialize (N.of_nat n).
+Definition nat_serialize n : IOStreamWriter.t := serialize (N.of_nat n).
 
-  Definition nat_deserialize : Reader.t nat := N.to_nat <$> deserialize.
+Definition nat_deserialize : ByteListReader.t nat := N.to_nat <$> deserialize.
 
 
-  (* This proof is typical for serializers defined by converting to and from a
+(* This proof is typical for serializers defined by converting to and from a
    type that is already serializable. Unfold the serializer and deserializer,
    call serialize_deserialize_id_crush, and then use the proof that the
    conversion functions are inverses. *)
-  Lemma nat_serialize_deserialize_id :
-    serialize_deserialize_id_spec nat_serialize nat_deserialize.
-  Proof.
-    unfold nat_serialize, nat_deserialize.
-    cheerios_crush.
-    now rewrite Nnat.Nat2N.id.
-  Qed.
+Lemma nat_serialize_deserialize_id :
+  serialize_deserialize_id_spec nat_serialize nat_deserialize.
+Proof.
+  unfold nat_serialize, nat_deserialize.
+  cheerios_crush.
+  now rewrite Nnat.Nat2N.id.
+Qed.
 
-  Instance nat_Serializer : Serializer nat.
-  Proof.
-    exact {| serialize := nat_serialize;
-             deserialize := nat_deserialize;
-             serialize_deserialize_id := nat_serialize_deserialize_id
-          |}.
-  Qed.
+Instance nat_Serializer : Serializer nat.
+Proof.
+  exact {| serialize := nat_serialize;
+           deserialize := nat_deserialize;
+           serialize_deserialize_id := nat_serialize_deserialize_id
+        |}.
+Qed.
 
-  (* Serializer for the standard library's Fin.t based on converting to nat. *)
-  Definition Fin_serialize {n} (x : Fin.t n) : Writer.t :=
-    serialize (proj1_sig (Fin.to_nat x)).
+(* Serializer for the standard library's Fin.t based on converting to nat. *)
+Definition Fin_serialize {n} (x : Fin.t n) : IOStreamWriter.t :=
+  serialize (proj1_sig (Fin.to_nat x)).
 
-  Definition Fin_deserialize {n} : Reader.t (Fin.t n) :=
-    m <- deserialize ;;
-      match Fin.of_nat m n with
-      | inleft x => Reader.ret x
-      | inright _ => Reader.error
-      end.
+Definition Fin_deserialize {n} : ByteListReader.t (Fin.t n) :=
+  m <- deserialize ;;
+    match Fin.of_nat m n with
+    | inleft x => ByteListReader.ret x
+    | inright _ => ByteListReader.error
+    end.
 
-  Lemma Fin_of_nat_to_nat:
-    forall (n : nat) (a : Fin.t n), Fin.of_nat (proj1_sig (Fin.to_nat a)) n = inleft a.
-  Proof.
-    induction a.
-    - auto.
-    - simpl. break_let. simpl in *.
-      now rewrite IHa.
-  Qed.
+Lemma Fin_of_nat_to_nat:
+  forall (n : nat) (a : Fin.t n), Fin.of_nat (proj1_sig (Fin.to_nat a)) n = inleft a.
+Proof.
+  induction a.
+  - auto.
+  - simpl. break_let. simpl in *.
+    now rewrite IHa.
+Qed.
 
-  Lemma Fin_serialize_deserialize_id n :
-    serialize_deserialize_id_spec Fin_serialize (@Fin_deserialize n).
-  Proof.
-    unfold Fin_serialize, Fin_deserialize.
-    cheerios_crush.
-    rewrite Fin_of_nat_to_nat.
-    cheerios_crush.
-  Qed.
+Lemma Fin_serialize_deserialize_id n :
+  serialize_deserialize_id_spec Fin_serialize (@Fin_deserialize n).
+Proof.
+  unfold Fin_serialize, Fin_deserialize.
+  cheerios_crush.
+  rewrite Fin_of_nat_to_nat.
+  cheerios_crush.
+Qed.
 
-  Instance Fin_Serializer n : Serializer (Fin.t n) :=
-    {| serialize := Fin_serialize;
-       deserialize := Fin_deserialize;
-       serialize_deserialize_id := Fin_serialize_deserialize_id n
-    |}.
+Instance Fin_Serializer n : Serializer (Fin.t n) :=
+  {| serialize := Fin_serialize;
+     deserialize := Fin_deserialize;
+     serialize_deserialize_id := Fin_serialize_deserialize_id n
+  |}.
 
-  (* Serializer for StructTact's fin based on converting to nat. *)
-  Definition fin_serialize {n} (x : fin n) : Writer.t :=
-    serialize (fin_to_nat x).
+(* Serializer for StructTact's fin based on converting to nat. *)
+Definition fin_serialize {n} (x : fin n) : IOStreamWriter.t :=
+  serialize (fin_to_nat x).
 
-  Definition fin_deserialize {n} : Reader.t (fin n) :=
-    m <- deserialize ;;
-      match fin_of_nat m n with
-      | inleft x => Reader.ret x
-      | inright _ => Reader.error
-      end.
+Definition fin_deserialize {n} : ByteListReader.t (fin n) :=
+  m <- deserialize ;;
+    match fin_of_nat m n with
+    | inleft x => ByteListReader.ret x
+    | inright _ => ByteListReader.error
+    end.
 
-  Lemma fin_serialize_deserialize_id n :
-    serialize_deserialize_id_spec fin_serialize (@fin_deserialize n).
-  Proof.
-    unfold fin_serialize, fin_deserialize.
-    cheerios_crush.
-    rewrite fin_of_nat_fin_to_nat.
-    cheerios_crush.
-  Qed.
+Lemma fin_serialize_deserialize_id n :
+  serialize_deserialize_id_spec fin_serialize (@fin_deserialize n).
+Proof.
+  unfold fin_serialize, fin_deserialize.
+  cheerios_crush.
+  rewrite fin_of_nat_fin_to_nat.
+  cheerios_crush.
+Qed.
 
-  Instance fin_Serializer n : Serializer (fin n) :=
-    {| serialize := fin_serialize;
-       deserialize := fin_deserialize;
-       serialize_deserialize_id := fin_serialize_deserialize_id n
-    |}.
+Instance fin_Serializer n : Serializer (fin n) :=
+  {| serialize := fin_serialize;
+     deserialize := fin_deserialize;
+     serialize_deserialize_id := fin_serialize_deserialize_id n
+  |}.
 
-  Definition ascii_serialize (a : Ascii.ascii) : Writer.t :=
-    serialize (Ascii.nat_of_ascii a).
+Definition ascii_serialize (a : Ascii.ascii) : IOStreamWriter.t :=
+  serialize (Ascii.nat_of_ascii a).
 
-  Definition ascii_deserialize : Reader.t Ascii.ascii :=
-    Ascii.ascii_of_nat <$> deserialize.
+Definition ascii_deserialize : ByteListReader.t Ascii.ascii :=
+  Ascii.ascii_of_nat <$> deserialize.
 
-  Lemma ascii_serialize_deserialize_id :
-    serialize_deserialize_id_spec ascii_serialize ascii_deserialize.
-  Proof.
-    unfold ascii_deserialize, ascii_serialize.
-    cheerios_crush.
-    now rewrite Ascii.ascii_nat_embedding.
-  Qed.
+Lemma ascii_serialize_deserialize_id :
+  serialize_deserialize_id_spec ascii_serialize ascii_deserialize.
+Proof.
+  unfold ascii_deserialize, ascii_serialize.
+  cheerios_crush.
+  now rewrite Ascii.ascii_nat_embedding.
+Qed.
 
-  Instance ascii_Serializer : Serializer Ascii.ascii :=
-    {| serialize := ascii_serialize;
-       deserialize := ascii_deserialize;
-       serialize_deserialize_id := ascii_serialize_deserialize_id
-    |}.
-End BasicSerializers.
+Instance ascii_Serializer : Serializer Ascii.ascii :=
+  {| serialize := ascii_serialize;
+     deserialize := ascii_deserialize;
+     serialize_deserialize_id := ascii_serialize_deserialize_id
+  |}.
+
