core/DeserializerMonad.v
@@ -1,40 +1,38 @@
+Require Import Cheerios.Core.
 Require Import Cheerios.Types.
 Require Import List.
 Import ListNotations.
 
-Module DeserializerMonad (Reader : READER).
-  Definition sequence {A B} (df : Reader.t (A -> B))
-             (da : Reader.t A) : Reader.t B :=
-    Reader.bind df
-                (fun f =>
-                   (Reader.bind da
-                                (fun a => Reader.ret (f a)))).
+Definition sequence {A B} (df : ByteListReader.t (A -> B))
+           (da : ByteListReader.t A) : ByteListReader.t B :=
+  ByteListReader.bind df
+                      (fun f =>
+                         (ByteListReader.bind da
+                                              (fun a => ByteListReader.ret (f a)))).
 
-  Lemma sequence_rewrite : forall {A B : Type}
-                                  (df : Reader.t (A -> B))
-                                  (da : Reader.t A),
-      sequence df da =
-      Reader.bind df
-                  (fun f =>
-                     (Reader.bind da
-                                  (fun a => Reader.ret (f a)))).
-  Proof.
-    reflexivity.
-  Qed.
-  Hint Rewrite @sequence_rewrite : cheerios.
+Lemma sequence_rewrite : forall {A B : Type}
+                                (df : ByteListReader.t (A -> B))
+                                (da : ByteListReader.t A),
+    sequence df da =
+    ByteListReader.bind df
+                        (fun f =>
+                           (ByteListReader.bind da
+                                                (fun a => ByteListReader.ret (f a)))).
+Proof.
+  reflexivity.
+Qed.
+Hint Rewrite @sequence_rewrite : cheerios.
 
-  Module DeserializerNotations.
-    Notation "m >>= f" := (@Reader.bind _ _ m f) (at level 42, left associativity).
+Module DeserializerNotations.
+  Notation "m >>= f" := (@ByteListReader.bind _ _ m f) (at level 42, left associativity).
 
-    Notation "x <- c1 ;; c2" := (c1 >>= (fun x => c2))
-                                  (at level 100, c1 at next level, right associativity).
-    Notation "e1 ;; e2" := (_ <- e1 ;; e2)
-                             (at level 100, right associativity).
+  Notation "x <- c1 ;; c2" := (c1 >>= (fun x => c2))
+                                (at level 100, c1 at next level, right associativity).
+  Notation "e1 ;; e2" := (_ <- e1 ;; e2)
+                           (at level 100, right associativity).
 
-    Notation "f <$> x" := (@Reader.map _ _ f x) (at level 42, left associativity).
+  Notation "f <$> x" := (@ByteListReader.map _ _ f x) (at level 42, left associativity).
 
-    Notation "f <*> x" := (@sequence _ _ f x) (at level 42, left associativity).
-  End DeserializerNotations.
+  Notation "f <*> x" := (@sequence _ _ f x) (at level 42, left associativity).
+End DeserializerNotations.
 
-  Import DeserializerNotations.
-End DeserializerMonad.
