core/Tactics.v
@@ -1,18 +1,13 @@
 Require Import List.
 
+Require Import Cheerios.Core.
 Require Import Cheerios.DeserializerMonad.
-Require Import Cheerios.IOStream.
 Require Import Cheerios.Types.
 
 Ltac cheerios_crush := intros; autorewrite with cheerios; auto.
 
-Module WriterRewrite (Writer : WRITER).
-  Hint Rewrite app_ass 
-       Writer.empty_unwrap Writer.putByte_unwrap
-       Writer.append_unwrap : cheerios.
-End WriterRewrite.
-
-Module ReaderRewrite (Reader : READER).
-  Hint Rewrite Reader.getByte_unwrap Reader.bind_unwrap Reader.ret_unwrap
-       Reader.map_unwrap @Reader.fold_unwrap : cheerios.
-End ReaderRewrite.
+Hint Rewrite app_ass
+     IOStreamWriter.empty_unwrap IOStreamWriter.putByte_unwrap
+     IOStreamWriter.append_unwrap
+     ByteListReader.getByte_unwrap ByteListReader.bind_unwrap ByteListReader.ret_unwrap
+     ByteListReader.map_unwrap @ByteListReader.fold_unwrap : cheerios.
