extraction/ExtrIOStream.v
@@ -3,26 +3,22 @@ Require Import ZArith.
 Require Import Cheerios.BasicSerializers.
 Require Import Cheerios.Core.
 Require Import Cheerios.Types.
-Require Import Cheerios.IOStream.
 
 Extract Constant
-        IOStream.t => "Iostream_primitives.serializer".
+        IOStreamWriter.t => "Iostream_primitives.serializer".
 Extract Constant
-        IOStream.wire => "Iostream_primitives.wire".
+        IOStreamWriter.wire => "Iostream_primitives.wire".
 
-Extract Constant IOStream.putByte => "Iostream_primitives.putByte".
-Extract Constant IOStream.empty => "Iostream_primitives.empty".
-Extract Constant IOStream.append => "Iostream_primitives.append".
-Extract Constant IOStream.wire_wrap => "Iostream_primitives.wire_wrap".
-Extract Constant IOStream.wire_eq_dec => "(=)".
+Extract Constant IOStreamWriter.putByte => "Iostream_primitives.putByte".
+Extract Constant IOStreamWriter.empty => "Iostream_primitives.empty".
+Extract Constant IOStreamWriter.append => "Iostream_primitives.append".
+Extract Constant IOStreamWriter.wire_wrap => "Iostream_primitives.wire_wrap".
+Extract Constant IOStreamWriter.wire_eq_dec => "(=)".
 
-Extract Constant IOStream.empty_unwrap => "Obj.magic".
-Extract Constant IOStream.putByte_unwrap => "Obj.magic".
-Extract Constant IOStream.append_unwrap => "Obj.magic".
-Extract Constant IOStream.wire_wrap_unwrap => "Obj.magic".
+Extract Constant IOStreamWriter.empty_unwrap => "Obj.magic".
+Extract Constant IOStreamWriter.putByte_unwrap => "Obj.magic".
+Extract Constant IOStreamWriter.append_unwrap => "Obj.magic".
+Extract Constant IOStreamWriter.wire_wrap_unwrap => "Obj.magic".
 
-Extract Constant IOStream.unwrap => "Obj.magic".
-Extract Constant IOStream.wire_unwrap => "Obj.magic".
-
-Extract Inlined Constant IOStreamSerializer.deserialize_top =>
-"Serializer_primitives.deserialize_top".
+Extract Constant IOStreamWriter.unwrap => "Obj.magic".
+Extract Constant IOStreamWriter.wire_unwrap => "Obj.magic".
