runtime/coq/ExtractPositiveSerializer.v
@@ -1,26 +1,16 @@
 Require Import Cheerios.ExtractPositiveSerializerDeps.
-Require Import Cheerios.IOStream.
 
 Require Import ZArith.
 Require Import ExtrOcamlBasic.
 Require Import ExtrOcamlString.
 
-Module ByteListBasics := BasicSerializers ByteListWriter ByteListReader ByteListSerializer.
-Module IOStreamBasics := BasicSerializers IOStream ByteListReader IOStreamSerializer.
+ Definition positive_serialize_top : positive -> IOStreamWriter.wire :=
+   serialize_top serialize.
 
-Definition positive_serialize_bytelist_top : positive -> ByteListWriter.wire :=
-  ByteListSerializer.serialize_top ByteListSerializer.serialize.
-
-Definition positive_deserialize_bytelist_top : ByteListWriter.wire -> option positive :=
-  ByteListSerializer.deserialize_top ByteListSerializer.deserialize.
-
-Definition positive_serialize_iostream_top : positive -> IOStream.wire :=
-  IOStreamSerializer.serialize_top IOStreamSerializer.serialize.
-
-Definition positive_deserialize_iostream_top : IOStream.wire -> option positive :=
-  IOStreamSerializer.deserialize_top IOStreamSerializer.deserialize.
+Definition positive_deserialize_top : IOStreamWriter.wire -> option positive :=
+  deserialize_top deserialize.
 
 Extraction "runtime/ocaml/positive_serializer.ml"
-           positive_serialize_bytelist_top positive_deserialize_bytelist_top
-           positive_serialize_iostream_top positive_deserialize_iostream_top.
+           positive_serialize_top positive_deserialize_top.
+
 
