runtime/coq/ExtractTreeSerializerDeps.v
@@ -2,6 +2,5 @@ Require Export Cheerios.Tree.
 Require Export Cheerios.Core.
 Require Export Cheerios.Types.
 Require Export Cheerios.ExtrByteListReader.
-Require Export Cheerios.ExtrByteListWriter.
 Require Export Cheerios.ExtrCheerios.
 Require Export Cheerios.ExtrIOStream.
